fstar/MLS.TreeSync.ParentHash.fst
@@ -20,6 +20,7 @@ type parent_hash_input_nt (bytes:Type0) {|bytes_like bytes|} (tkt:treekem_types 
 
 %splice [ps_parent_hash_input_nt] (gen_parser (`parent_hash_input_nt))
 %splice [ps_parent_hash_input_nt_length] (gen_length_lemma (`parent_hash_input_nt))
+%splice [ps_parent_hash_input_nt_is_valid] (gen_is_valid_lemma (`parent_hash_input_nt))
 
 instance parseable_serializeable_parent_hash_input_nt (bytes:Type0) {|bytes_like bytes|} (tkt:treekem_types bytes): parseable_serializeable bytes (parent_hash_input_nt bytes tkt) =
   mk_parseable_serializeable (ps_parent_hash_input_nt tkt)
